Weidenbach_Book/Watched_Literals_Watch_List_Code_Common.thy
@@ -184,10 +184,7 @@ abbreviation ann_lits_wl_assn :: \<open>ann_lits_wl \<Rightarrow> ann_lits_wl \<
 
 abbreviation clause_ll_assn :: \<open>nat clause_l \<Rightarrow> clause_wl \<Rightarrow> assn\<close> where
   \<open>clause_ll_assn \<equiv> array_assn unat_lit_assn\<close>
-(* TODO
-abbreviation clauses_ll_assn :: \<open>nat clauses_l \<Rightarrow> clauses_wl \<Rightarrow> assn\<close> where
-  \<open>clauses_ll_assn \<equiv> arlO_assn clause_ll_assn\<close>
-*)
+
 abbreviation clause_l_assn :: \<open>nat clause \<Rightarrow> uint32 list \<Rightarrow> assn\<close> where
   \<open>clause_l_assn \<equiv> list_mset_assn unat_lit_assn\<close>
 
@@ -269,109 +266,6 @@ proof -
         br_def Collect_eq_comp uint32_nat_rel_def dvd_div_eq_iff unat_lit_rel_def
       split: if_splits)+
 qed
-
-definition delete_index_and_swap_ll where
-  \<open>delete_index_and_swap_ll xs i j =
-     xs[i:= delete_index_and_swap (xs!i) j]\<close>
-
-definition delete_index_and_swap_aa where
-  \<open>delete_index_and_swap_aa xs i j = do {
-     x \<leftarrow> last_aa xs i;
-     xs \<leftarrow> update_aa xs i j x;
-     set_butlast_aa xs i
-  }\<close>
-
-
-lemma delete_index_and_swap_aa_ll_hnr[sepref_fr_rules]:
-  assumes \<open>is_pure R\<close>
-  shows \<open>(uncurry2 delete_index_and_swap_aa, uncurry2 (RETURN ooo delete_index_and_swap_ll))
-     \<in> [\<lambda>((l,i), j). i < length l \<and> j < length_ll l i]\<^sub>a (arrayO_assn (arl_assn R))\<^sup>d *\<^sub>a nat_assn\<^sup>k *\<^sub>a nat_assn\<^sup>k
-         \<rightarrow> (arrayO_assn (arl_assn R))\<close>
-  using assms unfolding delete_index_and_swap_aa_def
-  by sepref_to_hoare (sep_auto dest: le_length_ll_nemptyD
-      simp: delete_index_and_swap_ll_def update_ll_def last_ll_def set_butlast_ll_def
-      length_ll_def[symmetric])
-
-
-lemma nth_nat_of_uint32_nth': \<open>Array.nth x (nat_of_uint32 L) = Array.nth' x (integer_of_uint32 L)\<close>
-  by (auto simp: Array.nth'_def nat_of_uint32_code)
-
-lemma nth_aa_u_code[code]:
-  \<open>nth_aa_u x L L' = nth_u_code x L \<bind> (\<lambda>x. arl_get x L' \<bind> return)\<close>
-  unfolding nth_aa_u_def nth_aa_def arl_get_u_def[symmetric]  Array.nth'_def[symmetric]
-   nth_nat_of_uint32_nth' nth_u_code_def[symmetric] ..
-
-definition last_aa_u where
-  \<open>last_aa_u xs i = last_aa xs (nat_of_uint32 i)\<close>
-
-lemma last_aa_u_code[code]:
-  \<open>last_aa_u xs i = nth_u_code xs i \<bind> arl_last\<close>
-  unfolding last_aa_u_def last_aa_def nth_nat_of_uint32_nth' nth_nat_of_uint32_nth'
-    arl_get_u_def[symmetric] nth_u_code_def[symmetric] ..
-
-definition update_aa_u where
-  \<open>update_aa_u xs i j = update_aa xs (nat_of_uint32 i) j\<close>
-
-lemma Array_upd_upd': \<open>Array.upd i x a = Array.upd' a (of_nat i) x \<then> return a\<close>
-  by (auto simp: Array.upd'_def upd_return)
-
-definition Array_upd_u where
-  \<open>Array_upd_u i x a = Array.upd (nat_of_uint32 i) x a\<close>
-
-
-lemma Array_upd_u_code[code]: \<open>Array_upd_u i x a = heap_array_set'_u a i x \<then> return a\<close>
-  unfolding Array_upd_u_def heap_array_set'_u_def
-  Array.upd'_def
-  by (auto simp: nat_of_uint32_code upd_return)
-
-
-lemma update_aa_u_code[code]:
-  \<open>update_aa_u a i j y = do {
-      x \<leftarrow> nth_u_code a i;
-      a' \<leftarrow> arl_set x j y;
-      Array_upd_u i a' a
-    }\<close> -- \<open>is the Array.upd really needed?\<close>
-  unfolding update_aa_u_def update_aa_def nth_nat_of_uint32_nth' nth_nat_of_uint32_nth'
-    arl_get_u_def[symmetric] nth_u_code_def[symmetric]
-    heap_array_set'_u_def[symmetric] Array_upd_u_def[symmetric]
-  by auto
-
-definition set_butlast_aa_u where
-  \<open>set_butlast_aa_u xs i = set_butlast_aa xs (nat_of_uint32 i)\<close>
-
-lemma set_butlast_aa_u_code[code]:
-  \<open>set_butlast_aa_u a i = do {
-      x \<leftarrow> nth_u_code a i;
-      a' \<leftarrow> arl_butlast x;
-      Array_upd_u i a' a
-    }\<close> -- \<open>Replace the \<^term>\<open>i\<close>-th element by the itself execpt the last element.\<close>
-  unfolding set_butlast_aa_u_def set_butlast_aa_def
-   nth_u_code_def Array_upd_u_def
-  by (auto simp: Array.nth'_def nat_of_uint32_code)
-
-
-definition delete_index_and_swap_aa_u where
-   \<open>delete_index_and_swap_aa_u xs i = delete_index_and_swap_aa xs (nat_of_uint32 i)\<close>
-
-lemma delete_index_and_swap_aa_u_code[code]:
-\<open>delete_index_and_swap_aa_u xs i j = do {
-     x \<leftarrow> last_aa_u xs i;
-     xs \<leftarrow> update_aa_u xs i j x;
-     set_butlast_aa_u xs i
-  }\<close>
-  unfolding delete_index_and_swap_aa_u_def delete_index_and_swap_aa_def
-   last_aa_u_def update_aa_u_def set_butlast_aa_u_def
-  by auto
-
-lemma delete_index_and_swap_aa_ll_hnr_u[sepref_fr_rules]:
-  assumes \<open>is_pure R\<close>
-  shows \<open>(uncurry2 delete_index_and_swap_aa_u, uncurry2 (RETURN ooo delete_index_and_swap_ll))
-     \<in> [\<lambda>((l,i), j). i < length l \<and> j < length_ll l i]\<^sub>a (arrayO_assn (arl_assn R))\<^sup>d *\<^sub>a uint32_nat_assn\<^sup>k *\<^sub>a nat_assn\<^sup>k
-         \<rightarrow> (arrayO_assn (arl_assn R))\<close>
-  using assms unfolding delete_index_and_swap_aa_def delete_index_and_swap_aa_u_def
-  by sepref_to_hoare (sep_auto dest: le_length_ll_nemptyD
-      simp: delete_index_and_swap_ll_def update_ll_def last_ll_def set_butlast_ll_def
-      length_ll_def[symmetric] uint32_nat_rel_def br_def)
 
 
 subsection \<open>Code Generation\<close>
